library/init/data/quot.lean
@@ -16,13 +16,13 @@ attribute [subst]
 lemma iff_subst {a b : Prop} {p : Prop → Prop} (h₁ : a ↔ b) (h₂ : p a) : p b :=
 eq.subst (propext h₁) h₂
 
-constant quotient (α : Sort u) [setoid α] : Sort u
-protected constant quotient.mk {α : Sort u} [setoid α] : α → quotient α
+constant quotient {α : Sort u} (s : setoid α) : Sort u
+protected constant quotient.mk {α : Sort u} [s : setoid α] : α → quotient s
 protected axiom quotient.sound : ∀ {α : Sort u} [s : setoid α] {a b : α}, a ≈ b → quotient.mk a = quotient.mk b
-protected constant quotient.rec {α : Sort u} [setoid α] {β : quotient α → Sort v}
+protected constant quotient.rec {α : Sort u} [s : setoid α] {β : quotient s → Sort v}
     (f : ∀ a, β (quotient.mk a)) (h : ∀ a b, ∀ hs: a ≈ b, f a == f b) : ∀ q, β q
 
-computation_rule quotient.comp_rule {α : Sort u} (a : α) [setoid α] {β : quotient α → Sort v}
+computation_rule quotient.comp_rule {α : Sort u} (a : α) [s : setoid α] {β : quotient s → Sort v}
     (f : ∀ a, β (quotient.mk a)) (h) : quotient.rec f h (quotient.mk a) = f a
 
 attribute [elab_as_eliminator] quotient.rec
@@ -41,37 +41,37 @@ namespace quotient
 notation `⟦`:max a `⟧`:0 := quotient.mk a
 
 attribute [reducible, elab_as_eliminator]
-protected def lift {α : Sort u} {β : Sort v} [s : setoid α] (f : α → β) : (∀ a b, a ≈ b → f a = f b) → quotient α → β
+protected def lift {α : Sort u} {β : Sort v} [s : setoid α] (f : α → β) : (∀ a b, a ≈ b → f a = f b) → quotient s → β
 | h q := quotient.rec f (λ a b hs, heq_of_eq (h a b hs)) q
 
 attribute [elab_as_eliminator]
-protected lemma ind {α : Sort u} [setoid α] {β : quotient α → Prop} : (∀ a, β ⟦a⟧) → ∀ q, β q
+protected lemma ind {α : Sort u} [s : setoid α] {β : quotient s → Prop} : (∀ a, β ⟦a⟧) → ∀ q, β q
 | h q := quotient.rec h (λ a b hs, heq_of_eq_rec_left (quotient.sound hs) rfl) q
 
 attribute [reducible, elab_as_eliminator]
-protected def lift_on {α : Sort u} {β : Sort v} [setoid α] (q : quotient α) (f : α → β) (c : ∀ a b, a ≈ b → f a = f b) : β :=
+protected def lift_on {α : Sort u} {β : Sort v} [s : setoid α] (q : quotient s) (f : α → β) (c : ∀ a b, a ≈ b → f a = f b) : β :=
 quotient.lift f c q
 
 attribute [elab_as_eliminator]
-protected lemma induction_on {α : Sort u} [s : setoid α] {β : quotient α → Prop} (q : quotient α) (h : ∀ a, β ⟦a⟧) : β q :=
+protected lemma induction_on {α : Sort u} [s : setoid α] {β : quotient s → Prop} (q : quotient s) (h : ∀ a, β ⟦a⟧) : β q :=
 quotient.ind h q
 
-lemma exists_rep {α : Sort u} [s : setoid α] (q : quotient α) : ∃ a : α, ⟦a⟧ = q :=
+lemma exists_rep {α : Sort u} [s : setoid α] (q : quotient s) : ∃ a : α, ⟦a⟧ = q :=
 quotient.induction_on q (λ a, ⟨a, rfl⟩)
 
 section
 variable {α : Sort u}
 variable [s : setoid α]
-variable {β : quotient α → Sort v}
+variable {β : quotient s → Sort v}
 
 attribute [reducible, elab_as_eliminator]
 protected def rec_on
-   (q : quotient α) (f : Π a, β ⟦a⟧) (h : ∀ (a b : α) (p : a ≈ b), f a == f b) : β q :=
+   (q : quotient s) (f : Π a, β ⟦a⟧) (h : ∀ (a b : α) (p : a ≈ b), f a == f b) : β q :=
 quotient.rec f h q
 
 attribute [reducible, elab_as_eliminator]
 protected def rec_on_subsingleton
-   [h : ∀ a, subsingleton (β ⟦a⟧)] (q : quotient α) (f : Π a, β ⟦a⟧) : β q :=
+   [h : ∀ a, subsingleton (β ⟦a⟧)] (q : quotient s) (f : Π a, β ⟦a⟧) : β q :=
 quotient.rec_on q f (λ a b hs, subsingleton.helim (quotient.sound hs ▸ rfl) _ _)
 
 end
@@ -85,12 +85,12 @@ include s₁ s₂
 attribute [reducible, elab_as_eliminator]
 protected def lift₂
    (f : α → β → φ)(c : ∀ a₁ a₂ b₁ b₂, a₁ ≈ b₁ → a₂ ≈ b₂ → f a₁ a₂ = f b₁ b₂)
-   (q₁ : quotient α) (q₂ : quotient β) : φ :=
+   (q₁ : quotient s₁) (q₂ : quotient s₂) : φ :=
 quotient.lift
   (λ (a₁ : α), quotient.lift (f a₁) (λ (a b : β), c a₁ a a₁ b (setoid.refl a₁)) q₂)
   (λ (a b : α) (h : a ≈ b),
      @quotient.ind β s₂
-       (λ (a_1 : quotient β),
+       (λ (a_1 : quotient _),
           (quotient.lift (f a) (λ (a_1 b : β), c a a_1 a b (setoid.refl a)) a_1)
           =
           (quotient.lift (f b) (λ (a b_1 : β), c b a b b_1 (setoid.refl b)) a_1))
@@ -100,22 +100,22 @@ quotient.lift
 
 attribute [reducible, elab_as_eliminator]
 protected def lift_on₂
-  (q₁ : quotient α) (q₂ : quotient β) (f : α → β → φ) (c : ∀ a₁ a₂ b₁ b₂, a₁ ≈ b₁ → a₂ ≈ b₂ → f a₁ a₂ = f b₁ b₂) : φ :=
+  (q₁ : quotient s₁) (q₂ : quotient s₂) (f : α → β → φ) (c : ∀ a₁ a₂ b₁ b₂, a₁ ≈ b₁ → a₂ ≈ b₂ → f a₁ a₂ = f b₁ b₂) : φ :=
 quotient.lift₂ f c q₁ q₂
 
 attribute [elab_as_eliminator]
-protected lemma ind₂ {φ : quotient α → quotient β → Prop} (h : ∀ a b, φ ⟦a⟧ ⟦b⟧) (q₁ : quotient α) (q₂ : quotient β) : φ q₁ q₂ :=
+protected lemma ind₂ {φ : quotient s₁ → quotient s₂ → Prop} (h : ∀ a b, φ ⟦a⟧ ⟦b⟧) (q₁ : quotient s₁) (q₂ : quotient s₂) : φ q₁ q₂ :=
 quotient.ind (λ a₁, quotient.ind (λ a₂, h a₁ a₂) q₂) q₁
 
 attribute [elab_as_eliminator]
 protected lemma induction_on₂
-   {φ : quotient α → quotient β → Prop} (q₁ : quotient α) (q₂ : quotient β) (h : ∀ a b, φ ⟦a⟧ ⟦b⟧) : φ q₁ q₂ :=
+   {φ : quotient s₁ → quotient s₂ → Prop} (q₁ : quotient s₁) (q₂ : quotient s₂) (h : ∀ a b, φ ⟦a⟧ ⟦b⟧) : φ q₁ q₂ :=
 quotient.ind (λ a₁, quotient.ind (λ a₂, h a₁ a₂) q₂) q₁
 
 attribute [elab_as_eliminator]
 protected lemma induction_on₃
    [s₃ : setoid φ]
-   {δ : quotient α → quotient β → quotient φ → Prop} (q₁ : quotient α) (q₂ : quotient β) (q₃ : quotient φ) (h : ∀ a b c, δ ⟦a⟧ ⟦b⟧ ⟦c⟧)
+   {δ : quotient s₁ → quotient s₂ → quotient s₃ → Prop} (q₁ : quotient s₁) (q₂ : quotient s₂) (q₃ : quotient s₃) (h : ∀ a b c, δ ⟦a⟧ ⟦b⟧ ⟦c⟧)
    : δ q₁ q₂ q₃ :=
 quotient.ind (λ a₁, quotient.ind (λ a₂, quotient.ind (λ a₃, h a₁ a₂ a₃) q₃) q₂) q₁
 end
@@ -125,7 +125,7 @@ variable   {α : Sort u}
 variable   [s : setoid α]
 include s
 
-private def rel (q₁ q₂ : quotient α) : Prop :=
+private def rel (q₁ q₂ : quotient s) : Prop :=
 quotient.lift_on₂ q₁ q₂
   (λ a₁ a₂, a₁ ≈ a₂)
   (λ a₁ a₂ b₁ b₂ a₁b₁ a₂b₂,
@@ -135,10 +135,10 @@ quotient.lift_on₂ q₁ q₂
 
 local infix `~` := rel
 
-private lemma rel.refl : ∀ q : quotient α, q ~ q :=
+private lemma rel.refl : ∀ q : quotient s, q ~ q :=
 λ q, quotient.induction_on q (λ a, setoid.refl a)
 
-private lemma eq_imp_rel {q₁ q₂ : quotient α} : q₁ = q₂ → q₁ ~ q₂ :=
+private lemma eq_imp_rel {q₁ q₂ : quotient s} : q₁ = q₂ → q₁ ~ q₂ :=
 assume h, eq.rec_on h (rel.refl q₁)
 
 lemma exact {a b : α} : ⟦a⟧ = ⟦b⟧ → a ≈ b :=
@@ -153,8 +153,8 @@ include s₁ s₂
 
 attribute [reducible, elab_as_eliminator]
 protected def rec_on_subsingleton₂
-   {φ : quotient α → quotient β → Sort u_c} [h : ∀ a b, subsingleton (φ ⟦a⟧ ⟦b⟧)]
-   (q₁ : quotient α) (q₂ : quotient β) (f : Π a b, φ ⟦a⟧ ⟦b⟧) : φ q₁ q₂:=
+   {φ : quotient s₁ → quotient s₂ → Sort u_c} [h : ∀ a b, subsingleton (φ ⟦a⟧ ⟦b⟧)]
+   (q₁ : quotient s₁) (q₂ : quotient s₂) (f : Π a b, φ ⟦a⟧ ⟦b⟧) : φ q₁ q₂:=
 @quotient.rec_on_subsingleton _ s₁ (λ q, φ q q₂) (λ a, quotient.ind (λ b, h a b) q₂) q₁
   (λ a, quotient.rec_on_subsingleton q₂ (λ b, f a b))
 
@@ -162,8 +162,8 @@ end
 end quotient
 
 open decidable
-instance {α : Sort u} {s : setoid α} [d : ∀ a b : α, decidable (a ≈ b)] : decidable_eq (quotient α) :=
-λ q₁ q₂ : quotient α,
+instance {α : Sort u} {s : setoid α} [d : ∀ a b : α, decidable (a ≈ b)] : decidable_eq (quotient s) :=
+λ q₁ q₂,
   quotient.rec_on_subsingleton₂ q₁ q₂
     (λ a₁ a₂,
       match (d a₁ a₂) with
